instantiation prog and hopefully most of the fixes

theories/instantiation_func.v
@@ -6,8 +6,17 @@ From Coq Require Import BinNat.
 
 Section Instantiation_func.
 
-Import Interpreter_ctx_extract.
+Context `{ho: host}.
   
+Variable host_application_impl : host_state -> store_record -> function_type -> host_function -> seq value ->
+                       (host_state * option (store_record * result)).
+
+Hypothesis host_application_impl_correct :
+  (forall hs s ft hf vs hs' hres, (host_application_impl hs s ft hf vs = (hs', hres)) -> host_application hs s ft hf vs hs' hres).
+
+  (*
+Import Interpreter_ctx_extract.
+  *)
 Definition gather_m_f_type (tfs : list function_type) (m_f : module_func) : option function_type :=
   lookup_N tfs m_f.(modfunc_type).
 
@@ -29,15 +38,22 @@ Definition module_imports_typer (tfs: list function_type) (imps : list module_im
   those (map (fun imp => module_import_desc_typer tfs imp.(imp_desc)) imps).
 
 (* prepass *)
-Definition gather_m_e_type (tts: list table_type) (emode: module_elemmode) : option reference_type :=
-  match emode with
-  | ME_passive => Some T_funcref
-  | ME_active x offset => option_map tt_elem_type (lookup_N tts x)
-  | ME_declarative => Some T_funcref
+Definition gather_m_e_type (tts: list table_type) (el: module_element): option reference_type :=
+  match el.(modelem_mode) with
+  | ME_passive => Some el.(modelem_type)
+  | ME_active x offset =>
+      match option_map tt_elem_type (lookup_N tts x) with
+      | Some tref =>
+          if tref == el.(modelem_type)
+          then Some tref
+          else None
+      | None => None
+      end
+  | ME_declarative => Some el.(modelem_type)
   end.
 
 Definition gather_m_e_types (tts: list table_type) (els: list module_element) : option (list reference_type) :=
-  those (map (fun elem => gather_m_e_type tts elem.(modelem_mode)) els).
+  those (map (fun elem => gather_m_e_type tts elem) els).
 
 Definition gather_m_d_type (mts: list memory_type) (dmode: module_datamode) : option ok :=
   match dmode with
@@ -60,7 +76,7 @@ Definition module_exports_typer (c : t_context) exps :=
   those (map (fun exp => module_export_typer c exp.(modexp_desc)) exps).
 
 Definition gather_m_g_types (mgs : list module_global) : list global_type :=
-  List.map (fun mg => mg.(modglob_type)) mgs.
+  map (fun mg => mg.(modglob_type)) mgs.
 
 Definition module_func_type_checker (c : t_context) (m : module_func) : bool :=
   let '{| modfunc_type := i; modfunc_locals := t_locs; modfunc_body := b_es |} := m in
@@ -91,7 +107,7 @@ Definition module_global_type_checker (c : t_context) (mg : module_global) : boo
   const_exprs c es &&
   type_checker.b_e_type_checker c es (Tf nil [::tg.(tg_t)]).
 
-Definition module_elem_mode_checker (c: t_context) (emode: module_elemmode) (reftype: reference_type): bool :=
+Definition module_elem_mode_checker (c: t_context) (emode: module_elemmode) (reftype: reference_type) : bool :=
   match emode with
   | ME_passive => true
   | ME_active x offset =>
@@ -170,16 +186,16 @@ Definition module_type_checker (m : module) : option ((list extern_type) * (list
             |} in
     let c' := {|
       tc_types := nil;
-      tc_funcs := nil;
+      tc_funcs := c.(tc_funcs);
       tc_globals := igs;
-      tc_tables := tts;
-      tc_mems := mts;
-      tc_elems := rts;
-      tc_datas := dts;
+      tc_tables := c.(tc_tables);
+      tc_mems := c.(tc_mems);
+      tc_elems := nil;
+      tc_datas := nil;
       tc_locals := nil;
       tc_labels := nil;
       tc_return := None;
-      tc_refs := xs
+      tc_refs := c.(tc_refs)
     |} in
     if seq.all (module_func_type_checker c) fs &&
        seq.all (module_table_type_checker c) ts &&
@@ -187,7 +203,9 @@ Definition module_type_checker (m : module) : option ((list extern_type) * (list
        seq.all (module_global_type_checker c') gs &&
        seq.all (module_elem_type_checker c') els &&
        seq.all (module_data_type_checker c') ds &&
-       pred_option (module_start_type_checker c) i_opt then
+       pred_option (module_start_type_checker c) i_opt &&
+       export_name_unique exps
+      then
        match module_exports_typer c exps with
        | Some expts => Some (impts, expts)
        | None => None
@@ -198,11 +216,11 @@ Definition module_type_checker (m : module) : option ((list extern_type) * (list
   | (Some _, None) | (None, Some _) | (None, None) => None
   end.
 
-Definition external_type_checker (s : store_record) (v : extern_value) (e : extern_type) : bool :=
-  typing.ext_typing s v == Some e.
+Definition external_type_checker (s : store_record) (v : extern_value): option extern_type :=
+  typing.ext_typing s v.
 
-Definition interp_get_v (s : store_record) (f : frame) (b_es : list basic_instruction) : option value :=
-  match run_multi_step_raw tt 5 s f 1 (operations.to_e_list b_es) with
+Definition interp_get_v (hs: host_state) (s : store_record) (f : frame) (b_es : list basic_instruction) : option value :=
+  match run_multi_step_raw host_application_impl_correct hs 5 s f 1 (operations.to_e_list b_es) with
   | inr vs =>
     match vs with
     | [:: v] => Some v
@@ -211,53 +229,57 @@ Definition interp_get_v (s : store_record) (f : frame) (b_es : list basic_instru
   | _ => None
   end.
 
-Definition interp_get_vref (s : store_record) (f: frame) (b_es : list basic_instruction) : option value_ref :=
-  match interp_get_v s f b_es with
+Definition interp_get_vref (hs: host_state) (s : store_record) (f: frame) (b_es : list basic_instruction) : option value_ref :=
+  match interp_get_v hs s f b_es with
   | Some (VAL_ref vref) => Some vref
   | _ => None
   end.
 
-Definition interp_get_i32 (s : store_record) (f: frame) (b_es : list basic_instruction) : option i32 :=
-  match interp_get_v s f b_es with
+Definition interp_get_i32 (hs: host_state) (s : store_record) (f: frame) (b_es : list basic_instruction) : option i32 :=
+  match interp_get_v hs s f b_es with
   | Some (VAL_num (VAL_int32 c)) => Some c
   | _ => None
   end.
 
-Definition get_global_inits (s: store_record) (f: frame) (gs: list module_global) : option (list value):=
-  those (map (fun g => interp_get_v s f g.(modglob_init)) gs).
+Definition get_global_inits (hs: host_state) (s: store_record) (f: frame) (gs: list module_global) : option (list value):=
+  those (map (fun g => interp_get_v hs s f g.(modglob_init)) gs).
 
-Definition get_elem_inits (s: store_record) (f: frame) (els: list module_element) : option (list (list value_ref)):=
-  those (map (fun el => those (map (fun e => interp_get_vref s f e) el.(modelem_init))) els).
+Definition get_elem_inits (hs: host_state) (s: store_record) (f: frame) (els: list module_element) : option (list (list value_ref)):=
+  those (map (fun el => those (map (fun e => interp_get_vref hs s f e) el.(modelem_init))) els).
 
-Definition interp_instantiate (s : store_record) (m : module) (v_imps : list extern_value) : option ((store_record * frame * list basic_instruction)) :=
+Definition interp_instantiate (hs: host_state) (s : store_record) (m : module) (v_imps : list extern_value) : option ((host_state * store_record * frame * list basic_instruction)) :=
   match module_type_checker m with
   | None => None
-  | Some (t_imps, t_exps) =>
-      if all2 (external_type_checker s) v_imps t_imps then
-        let inst_init :=
-          {|
-            inst_types := nil;
-            inst_funcs := (ext_funcs v_imps) ++ (map N.of_nat (iota (length (s_funcs s)) (length (mod_funcs m))));
-            inst_tables := nil;
-            inst_mems := nil;
-            inst_globals := ext_globs v_imps;
-            inst_elems := nil;
-            inst_datas := nil;
-            inst_exports := nil;
-          |} in
-        let f_init := Build_frame nil inst_init in
-        match get_global_inits s f_init m.(mod_globals) with
-        | None => None
-        | Some g_inits =>
-            match get_elem_inits s f_init m.(mod_elems) with
-            | Some r_inits =>
-                let '(s', inst_final) := interp_alloc_module s m v_imps g_inits r_inits in
-                let f_final := Build_frame nil inst_final in
-                Some (s', f_final, get_init_expr_elems m.(mod_elems) ++ get_init_expr_datas m.(mod_datas) ++ get_init_expr_start m.(mod_start))
+  | Some (t_imps_mod, t_exps) =>
+      match those (map (external_type_checker s) v_imps) with
+      | Some t_imps =>
+          if all2 import_subtyping t_imps t_imps_mod then
+            let inst_init :=
+              {|
+                inst_types := nil;
+                inst_funcs := (ext_funcs v_imps) ++ (map N.of_nat (iota (length (s_funcs s)) (length (mod_funcs m))));
+                inst_tables := nil;
+                inst_mems := nil;
+                inst_globals := ext_globs v_imps;
+                inst_elems := nil;
+                inst_datas := nil;
+                inst_exports := nil;
+              |} in
+            let f_init := Build_frame nil inst_init in
+            match get_global_inits hs s f_init m.(mod_globals) with
             | None => None
+            | Some g_inits =>
+                match get_elem_inits hs s f_init m.(mod_elems) with
+                | Some r_inits =>
+                    let '(s', inst_final) := interp_alloc_module s m v_imps g_inits r_inits in
+                    let f_final := Build_frame nil inst_final in
+                    Some (hs, s', f_final, get_init_expr_elems m.(mod_elems) ++ get_init_expr_datas m.(mod_datas) ++ get_init_expr_start m.(mod_start))
+                | None => None
+                end
             end
-        end
-      else None
+          else None
+      | None => None
+      end
   end.
 
 Definition empty_store_record : store_record := {|
@@ -269,11 +291,19 @@ Definition empty_store_record : store_record := {|
     s_datas := nil;
   |}.
 
+End Instantiation_func.
+
+(** Extraction **)
+
+Module Instantiation_func_extract.
+
+Import Interpreter_ctx_extract.
+  
 (* Add an empty host and provide an initial empty store, and convert the 
    starting expression to administrative *)
 Definition interp_instantiate_wrapper (m : module) : option (host_state * store_record * frame * list administrative_instruction) :=
-  match interp_instantiate empty_store_record m nil with
-  | Some (s, i, bes) => Some (tt, s, i, to_e_list bes)
+  match interp_instantiate host_application_impl host_application_impl_correct tt empty_store_record m nil with
+  | Some (hs, s, i, bes) => Some (hs, s, i, to_e_list bes)
   | None => None
   end.
 
@@ -297,19 +327,5 @@ Definition lookup_exported_function (n : name) (s: store_record) (f: frame)
       end)
     f.(f_inst).(inst_exports)
     None.
-
-End Instantiation_func.
-
-(** Extraction **)
-
-Module Instantiation_func_extract.
-
-Definition lookup_exported_function : name -> store_record -> frame -> option (list administrative_instruction) :=
-  lookup_exported_function.
-
-Definition interp_instantiate_wrapper :
-  module ->
-  option (host_state * store_record * frame * list administrative_instruction) :=
-  interp_instantiate_wrapper.
 
 End Instantiation_func_extract.
